theories/Syntax/UntypedReduction.v
@@ -1,67 +1,76 @@
 (** * LogRel.Syntax.UntypedReduction: untyped reduction, used to define algorithmic typing.*)
 From Stdlib Require Import CRelationClasses.
 From LogRel Require Import Utils AutoSubst.Extra Notations.
-From LogRel.Syntax Require Import BasicAst Context NormalForms Weakening.
+From Equations Require Import Equations. (* for depelim *)
+From LogRel.Syntax Require Import BasicAst Context NormalForms Weakening Computations.
 
 (** ** Reductions *)
 
 (** *** One-step reduction. *)
 
-Inductive OneRedAlg : term -> term -> Type :=
+Inductive OneRedAlg {L : Fcontext} : term -> term -> Type :=
 | BRed {A a t} :
-    [ tApp (tLambda A t) a ⤳ t[a..] ]
+    [ L | tApp (tLambda A t) a ⤳ t[a..] ]
 | appSubst {t u a} :
-    [ t ⤳ u ] ->
-    [ tApp t a ⤳ tApp u a ]
+    [ L |t ⤳ u ] ->
+    [ L |tApp t a ⤳ tApp u a ]
 | natElimSubst {P hz hs n n'} :
-    [ n ⤳ n' ] ->
-    [ tNatElim P hz hs n ⤳ tNatElim P hz hs n' ]
+    [ L |n ⤳ n' ] ->
+    [ L |tNatElim P hz hs n ⤳ tNatElim P hz hs n' ]
 | natElimZero {P hz hs} :
-    [ tNatElim P hz hs tZero ⤳ hz ]
+    [ L |tNatElim P hz hs tZero ⤳ hz ]
 | natElimSucc {P hz hs n} :
-    [ tNatElim P hz hs (tSucc n) ⤳ tApp (tApp hs n) (tNatElim P hz hs n) ]
+    [ L |tNatElim P hz hs (tSucc n) ⤳ tApp (tApp hs n) (tNatElim P hz hs n) ]
 | boolElimSubst {P ht hf n n'} :
-    [ n ⤳ n' ] ->
-    [ tBoolElim P ht hf n ⤳ tBoolElim P ht hf n' ]
+    [ L |n ⤳ n' ] ->
+    [ L |tBoolElim P ht hf n ⤳ tBoolElim P ht hf n' ]
 | boolElimTrue {P ht hf} :
-    [ tBoolElim P ht hf tTrue ⤳ ht ]
+    [ L |tBoolElim P ht hf tTrue ⤳ ht ]
 | boolElimFalse {P ht hf} :
-    [ tBoolElim P ht hf tFalse ⤳ hf ]
+    [ L |tBoolElim P ht hf tFalse ⤳ hf ]
+| alphaSubst {n n'} :
+  [ L | n ⤳ n' ] -> [ L | tAlpha n ⤳ tAlpha n' ]
+| alphaSubstSucc {n n'} :
+  [ L | tAlpha n ⤳ tAlpha n' ] -> [ L | tAlpha (tSucc n) ⤳ tAlpha (tSucc n') ]
+| alphaRed {n b} : in_Fctx L n b ->
+  [ L | tAlpha (nat_to_term n) ⤳ bool_to_term b]
 | emptyElimSubst {P e e'} :
-    [e ⤳ e'] ->
-    [tEmptyElim P e ⤳ tEmptyElim P e']        
+    [L |e ⤳ e'] ->
+    [L |tEmptyElim P e ⤳ tEmptyElim P e']
 | fstSubst {p p'} :
-    [ p ⤳ p'] ->
-    [ tFst p ⤳ tFst p']
+    [ L |p ⤳ p'] ->
+    [ L |tFst p ⤳ tFst p']
 | fstPair {A B a b} :
-    [ tFst (tPair A B a b) ⤳ a ]
+    [ L |tFst (tPair A B a b) ⤳ a ]
 | sndSubst {p p'} :
-    [ p ⤳ p'] ->
-    [ tSnd p ⤳ tSnd p']
+    [ L |p ⤳ p'] ->
+    [ L |tSnd p ⤳ tSnd p']
 | sndPair {A B a b} :
-    [ tSnd (tPair A B a b) ⤳ b ]
+    [ L |tSnd (tPair A B a b) ⤳ b ]
 | idElimRefl {A x P hr y A' z} :
-  [ tIdElim A x P hr y (tRefl A' z) ⤳ hr ]
+  [ L |tIdElim A x P hr y (tRefl A' z) ⤳ hr ]
 | idElimSubst {A x P hr y e e'} :
-  [e ⤳ e'] ->
-  [ tIdElim A x P hr y e ⤳ tIdElim A x P hr y e' ]
+  [L |e ⤳ e'] ->
+  [ L |tIdElim A x P hr y e ⤳ tIdElim A x P hr y e' ]
 
-where "[ t ⤳ t' ]" := (OneRedAlg t t') : typing_scope.
+where "[ L | t ⤳ t' ]" := (@OneRedAlg L t t') : typing_scope.
 
 (* Keep in sync with OneRedTermDecl! *)
 
 (** *** Multi-step reduction *)
 
-Inductive RedClosureAlg : term -> term -> Type :=
+Inductive RedClosureAlg {L : Fcontext} : term -> term -> Type :=
   | redIdAlg {t} :
-    [ t ⤳* t ]
+    [ L | t ⤳* t ]
   | redSuccAlg {t t' u} :
-    [ t ⤳ t'] ->
-    [ t' ⤳* u ] ->
-    [ t ⤳* u ]
-  where "[ t ⤳* t' ]" := (RedClosureAlg t t') : typing_scope.
+    [ L | t ⤳ t'] ->
+    [ L | t' ⤳* u ] ->
+    [ L | t ⤳* u ]
+  where "[ L | t ⤳* t' ]" := (@RedClosureAlg L t t') : typing_scope.
 
-#[export] Instance RedAlgTrans : PreOrder RedClosureAlg.
+Equations Derive Signature for RedClosureAlg.
+
+#[export] Instance RedAlgTrans {L} : PreOrder (RedClosureAlg (L:=L)).
   Proof.
     split.
     - now econstructor.
@@ -75,7 +84,7 @@ Inductive RedClosureAlg : term -> term -> Type :=
 (** The symmetric of reduction, in Prop. The well-founded relation on which the reduction
   machine operates. *)
 
-Record cored t t' : Prop := { _ : [t' ⤳ t] }.
+Record cored L t t' : Prop := { _ : [L |t' ⤳ t] }.
 
 (** ** Properties *)
 
@@ -84,29 +93,45 @@ Record cored t t' : Prop := { _ : [t' ⤳ t] }.
 Ltac inv_whne :=
   match goal with [ H : whne _ |- _ ] => inversion H end.
 
-Lemma whne_nored n u :
-  whne n -> [n ⤳ u] -> False.
+Lemma whne_nored {L} n u :
+  whne n -> [ L | n ⤳ u] -> False.
 Proof.
   intros ne red.
   induction red in ne |- *.
-  all: inversion ne ; subst ; clear ne.
-  2: auto.
-  all: now inv_whne.
+  11: clear i; induction n.
+  all : inversion ne; subst; clear ne; try now inv_whne.
+  inversion red.
 Qed.
 
-Lemma whnf_nored n u :
-  whnf n -> [n ⤳ u] -> False.
+Lemma whnf_nored L n u :
+  whnf n -> [ L | n ⤳ u] -> False.
 Proof.
   intros nf red.
   induction red in nf |- *.
-  2,3,6,9,10,12,15: inversion nf; subst; inv_whne; subst; apply IHred; now constructor.
-  all: inversion nf; subst; inv_whne; subst; try now inv_whne.
+  2,3,6,9,12,13,15,18 : inversion nf; subst; inv_whne; subst; apply IHred; now constructor.
+  7:clear i; induction n.
+  1-11: inversion nf; subst; inv_whne; subst; try now inv_whne.
+  - apply IHred; now constructor.
+  - apply IHn; now constructor.
 Qed.
 
 (** *** Determinism of reduction *)
 
-Lemma ored_det {t u v} :
-  [t ⤳ u] -> [t ⤳ v] ->
+Lemma ored_detaux : forall {L n n'}, [ L | tAlpha (nat_to_term n) ⤳ tAlpha n'] -> False.
+Proof.
+  intros L n.
+  induction n; intros.
+  - inversion H; subst.
+    * inversion H2.
+    * destruct b; inversion H1.
+  - inversion H; subst.
+    * inversion H2.
+    * now apply IHn in H2.
+    * destruct b; inversion H1.
+Qed.
+
+Lemma ored_det {L t u v} :
+  [L | t ⤳ u] -> [L | t ⤳ v] ->
   u = v.
 Proof.
   intros red red'.
@@ -139,6 +164,24 @@ Proof.
   - inversion red'; try reflexivity; subst.
     exfalso; eapply whnf_nored; tea; constructor.
   - inversion red'; subst.
+    + f_equal; now apply IHred.
+    + inversion red.
+    + destruct n0; inversion red.
+  - inversion red'; subst.
+    + inversion H0.
+    + apply IHred in H0.
+      inversion H0; subst.
+      reflexivity.
+    + destruct n0; inversion H; subst.
+      destruct (ored_detaux red).
+  - inversion red'; subst.
+    + destruct (ored_detaux red').
+    + destruct (ored_detaux red').
+    + apply nat_to_term_inj in H.
+      destruct H.
+      f_equal.
+      now eapply functionality.
+  - inversion red'; subst.
     f_equal; eauto.
   - inversion red'; subst; clear red'.
     1: f_equal; now eapply IHred.
@@ -157,7 +200,7 @@ Proof.
     exfalso; eapply whnf_nored;tea; constructor.
 Qed.
 
-Lemma red_whne t u : [t ⤳* u] -> whne t -> t = u.
+Lemma red_whne {L} t u : [ L | t ⤳* u] -> whne t -> t = u.
 Proof.
   intros [] ?.
   1: reflexivity.
@@ -165,7 +208,7 @@ Proof.
   eauto using whne_nored.
 Qed.
 
-Lemma red_whnf t u : [t ⤳* u] -> whnf t -> t = u.
+Lemma red_whnf {L} t u : [L | t ⤳* u] -> whnf t -> t = u.
 Proof.
   intros [] ?.
   1: reflexivity.
@@ -173,10 +216,10 @@ Proof.
   eauto using whnf_nored.
 Qed.
 
-Lemma whred_red_det t u u' :
+Lemma whred_red_det {L} t u u' :
   whnf u ->
-  [t ⤳* u] -> [t ⤳* u'] ->
-  [u' ⤳* u].
+  [L | t ⤳* u] -> [L | t ⤳* u'] ->
+  [ L | u' ⤳* u].
 Proof.
   intros whnf red red'.
   induction red in whnf, u', red' |- *.
@@ -188,9 +231,9 @@ Proof.
       now eapply IHred.
 Qed.
 
-Corollary whred_det t u u' :
+Corollary whred_det {L} t u u' :
   whnf u -> whnf u' ->
-  [t ⤳* u] -> [t ⤳* u'] ->
+  [L | t ⤳* u] -> [L | t ⤳* u'] ->
   u = u'.
 Proof.
   intros.
@@ -200,21 +243,39 @@ Qed.
 
 (** *** Stability by weakening *)
 
-Lemma oredalg_wk (ρ : nat -> nat) (t u : term) :
-[t ⤳ u] ->
-[t⟨ρ⟩ ⤳ u⟨ρ⟩].
+Lemma oFredalg L L' t u: 
+  Fweakening L' L ->
+  [L | t ⤳ u] -> [L' | t ⤳ u].
+Proof.
+  intros hFwk hred.
+  induction hred.
+  all: now constructor.
+Defined.
+
+Lemma cFredalg L L' t u: 
+  Fweakening L' L ->
+  [L | t ⤳* u] -> [L' | t ⤳* u].
+Proof.
+  induction 2; econstructor; eauto using oFredalg.
+Defined.
+
+Lemma oredalg_wk (ρ : nat -> nat) L (t u : term) :
+  [L | t ⤳ u] ->
+  [L | t⟨ρ⟩ ⤳ u⟨ρ⟩].
 Proof.
   intros Hred.
   induction Hred in ρ |- *.
-  2-15: cbn; asimpl; now econstructor.
+  2-10,12-18: cbn; asimpl; now econstructor.
   - cbn ; asimpl.
     evar (t' : term).
     replace (subst_term _ t) with t'.
     all: subst t'.
     1: econstructor.
     now asimpl.
+  - asimpl. rewrite nat_to_term_ren. rewrite bool_to_term_ren.
+    now econstructor.
 Qed.
-
+(* 
 Lemma oredalg_str (Γ Δ : context) (ρ : Δ ≤ Γ) (t u : term) :
   [t⟨ρ⟩ ⤳ u] ->
   ∑ u', u = u'⟨ρ⟩ × [t ⤳ u'].
@@ -229,15 +290,22 @@ Proof.
   end.
   all: try (edestruct IHHred as [? [->]]; [reflexivity|..]).
   all: eexists ; split ; cycle -1 ; [now econstructor | now bsimpl].
-Qed.
+Qed. *)
 
-Lemma credalg_wk (ρ : nat -> nat) (t u : term) :
-[t ⤳* u] ->
-[t⟨ρ⟩ ⤳* u⟨ρ⟩].
+Lemma credalg_wk (ρ : nat -> nat) {L} (t u : term) :
+[L|t ⤳* u] ->
+[L|t⟨ρ⟩ ⤳* u⟨ρ⟩].
 Proof.
   induction 1 ; econstructor ; eauto using oredalg_wk.
 Qed.
 
+Lemma credalg_Fwk (Γ Δ : context) (ρ : Δ ≤ Γ) (t u : term) :
+[Γ|t ⤳* u] ->
+[Δ | t⟨ρ⟩ ⤳* u⟨ρ⟩].
+Proof.
+  intros. apply credalg_wk. destruct ρ. now eapply cFredalg.
+Qed.
+(* 
 Lemma credalg_str (Γ Δ : context) (ρ : Δ ≤ Γ) (t u : term) :
   [t⟨ρ⟩ ⤳* u] ->
   ∑ u', u = u'⟨ρ⟩ × [t ⤳* u'].
@@ -252,11 +320,11 @@ Proof.
     edestruct IHHred as [? [->]]; [reflexivity|..].
     eexists ; split ; [reflexivity|..].
     now econstructor.
-Qed.
+Qed. *)
 
 (** Derived rules *)
 
-Lemma redalg_app {t t' u} : [t ⤳* t'] -> [tApp t u ⤳* tApp t' u].
+Lemma redalg_app {L t t' u} : [ L | t ⤳* t'] -> [ L | tApp t u ⤳* tApp t' u].
 Proof.
 induction 1.
 + reflexivity.
@@ -264,7 +332,7 @@ induction 1.
   now econstructor.
 Qed.
 
-Lemma redalg_natElim {P hs hz t t'} : [t ⤳* t'] -> [tNatElim P hs hz t ⤳* tNatElim P hs hz t'].
+Lemma redalg_natElim {L P hs hz t t'} : [L | t ⤳* t'] -> [L|tNatElim P hs hz t ⤳* tNatElim P hs hz t'].
 Proof.
 induction 1.
 + reflexivity.
@@ -272,7 +340,7 @@ induction 1.
   now econstructor.
 Qed.
 
-Lemma redalg_boolElim {P ht hf t t'} : [t ⤳* t'] -> [tBoolElim P ht hf t ⤳* tBoolElim P ht hf t'].
+Lemma redalg_boolElim {L P ht hf t t'} : [ L | t ⤳* t'] -> [L|tBoolElim P ht hf t ⤳* tBoolElim P ht hf t'].
 Proof.
 induction 1.
 + reflexivity.
@@ -280,7 +348,7 @@ induction 1.
   now econstructor.
 Qed.
 
-Lemma redalg_emptyElim {P t t'} : [t ⤳* t'] -> [tEmptyElim P t ⤳* tEmptyElim P t'].
+Lemma redalg_emptyElim {L P t t'} : [L | t ⤳* t'] -> [L|tEmptyElim P t ⤳* tEmptyElim P t'].
 Proof.
 induction 1.
 + reflexivity.
@@ -288,28 +356,55 @@ induction 1.
   now econstructor.
 Qed.
 
-Lemma redalg_fst {t t'} : [t ⤳* t'] -> [tFst t ⤳* tFst t'].
+Lemma redalg_fst {L t t'} : [ L | t ⤳* t'] -> [L|tFst t ⤳* tFst t'].
 Proof.
   induction 1; [reflexivity|].
   econstructor; tea; now constructor.
 Qed.
 
-Lemma redalg_snd {t t'} : [t ⤳* t'] -> [tSnd t ⤳* tSnd t'].
+Lemma redalg_snd { L t t'} : [ L | t ⤳* t'] -> [L | tSnd t ⤳* tSnd t'].
 Proof.
   induction 1; [reflexivity|].
   econstructor; tea; now constructor.
 Qed.
 
-Lemma redalg_idElim {A x P hr y t t'} : [t ⤳* t'] -> [tIdElim A x P hr y t ⤳* tIdElim A x P hr y t'].
+Lemma redalg_idElim { L A x P hr y t t'} : [ L | t ⤳* t'] -> [L | tIdElim A x P hr y t ⤳* tIdElim A x P hr y t'].
 Proof.
   induction 1; [reflexivity|].
   econstructor; tea; now constructor.
 Qed.
 
-Lemma redalg_one_step {t t'} : [t ⤳ t'] -> [t ⤳* t'].
+Lemma redalg_alpha {L t t'} : [L | t ⤳* t'] -> [L | tAlpha t ⤳* tAlpha t'].
+Proof.
+  induction 1; [reflexivity|].
+  econstructor; tea; now econstructor.
+Qed.
+
+Lemma redalg_alphaSucc {L t t'} : [L | tAlpha t ⤳* tAlpha t'] -> [L | tAlpha (tSucc t) ⤳* tAlpha (tSucc t')].
+Proof.
+  intros hα.
+  change (match tAlpha t, tAlpha t' with
+    |tAlpha u, tAlpha u' => [L | tAlpha (tSucc u) ⤳* tAlpha (tSucc u')]
+    | _,_ => unit end).
+  induction hα; destruct t0; try apply tt; [reflexivity|destruct u]; try apply tt.
+  inversion o; subst.
+  - econstructor; tea; now econstructor.
+  - econstructor; tea; now econstructor.
+  - destruct b; inversion hα; subst; inversion H.
+Qed.
+
+Lemma redalg_alphanSucc {L t t' n} : [L | tAlpha t ⤳* tAlpha t'] -> [L | tAlpha (nSucc n t) ⤳* tAlpha (nSucc n t')].
+Proof.
+  induction n; intros.
+  - tea.
+  - eauto using redalg_alphaSucc.
+Qed.
+
+
+Lemma redalg_one_step {L t t'} : [ L | t ⤳ t'] -> [ L | t ⤳* t'].
 Proof. intros; econstructor;[tea|reflexivity]. Qed.
 
-Lemma eta_expand_beta {A t} : [(eta_expand (tLambda A t)) ⤳ t].
+Lemma eta_expand_beta { L A t} : [ L | (eta_expand (tLambda A t)) ⤳ t].
 Proof.
   cbn.
   evar (t' : term).
@@ -319,10 +414,10 @@ Proof.
   now bsimpl.
 Qed.
 
-Lemma eta_expand_beta_inv {A t t'} :
-  [tApp (tLambda A t)⟨↑⟩ (tRel 0) ⤳* t'] ->
+Lemma eta_expand_beta_inv {L A t t'} :
+  [L | tApp (tLambda A t)⟨↑⟩ (tRel 0) ⤳* t'] ->
   whnf t' ->
-  [t ⤳* t'].
+  [L | t ⤳* t'].
 Proof.
   intros red nf.
   inversion red ; subst ; clear red.
@@ -339,10 +434,10 @@ Proof.
 Qed.
 
 
-Lemma eta_expand_fst_inv {A B t u t'} :
-  [tFst (tPair A B t u) ⤳* t'] ->
+Lemma eta_expand_fst_inv {L A B t u t'} :
+  [L | tFst (tPair A B t u) ⤳* t'] ->
   whnf t' ->
-  [t ⤳* t'].
+  [L | t ⤳* t'].
 Proof.
   intros red nf.
   inversion red ; subst ; clear red.
@@ -356,10 +451,10 @@ Proof.
 Qed.
 
 
-Lemma eta_expand_snd_inv {A B t u u'} :
-  [tSnd (tPair A B t u) ⤳* u'] ->
+Lemma eta_expand_snd_inv {L A B t u u'} :
+  [L | tSnd (tPair A B t u) ⤳* u'] ->
   whnf u' ->
-  [u ⤳* u'].
+  [L|u ⤳* u'].
 Proof.
   intros red nf.
   inversion red ; subst ; clear red.
