theories/Validity/Irrelevance.v
@@ -2,6 +2,7 @@ From Stdlib Require Import CRelationClasses.
 From LogRel Require Import Utils Syntax.All GenericTyping LogicalRelation.
 From LogRel.LogicalRelation Require Import Properties.
 From LogRel.Validity Require Import Validity.
+From Equations Require Import Equations.
 
 Set Universe Polymorphism.
 Set Printing Primitive Projection Parameters.
@@ -13,14 +14,25 @@ Section VRIrrelevant.
 Universes u1 u2 u3 u4 v1 v2 v3 v4.
 
 Set Printing Universes.
-Lemma VRirrelevant@{} Γ Γ' {veqsubst : forall Δ (h :[|-Δ]) (σ σ' : nat -> term), Type@{u3}} {veqsubst' : forall Δ (h :[|-Δ]) (σ σ' : nat -> term), Type@{v3}}
+Lemma VRirrelevant@{} (Γ Γ':context) {veqsubst : forall Δ (h :[|-Δ]) {ρF : Fweakening Δ Γ} {ρF' : Fweakening Δ Γ'} (σ σ' : nat -> term), Type@{u3}} {veqsubst' : forall Δ (h :[|-Δ]) {ρF : Fweakening Δ Γ} {ρF' : Fweakening Δ Γ'} (σ σ' : nat -> term), Type@{v3}}
   (vr : VR@{u1 u2 u3 u4} Γ Γ' veqsubst) (vr' : VR@{v1 v2 v3 v4} Γ Γ'  veqsubst') :
-  (forall Δ σ σ' wfΔ wfΔ', veqsubst Δ  wfΔ σ σ' <~> veqsubst' Δ wfΔ' σ σ').
+  (forall (Δ:context) wfΔ wfΔ' {ρF : Fweakening Δ Γ} {ρF' : Fweakening Δ Γ'} σ σ', veqsubst Δ wfΔ σ σ' <~> veqsubst' Δ wfΔ' σ σ').
 Proof.
-  revert veqsubst' vr'.  pattern Γ, Γ', veqsubst, vr.
+  revert veqsubst' vr'. pattern Γ, Γ', veqsubst, vr.
   apply VR_rect; clear Γ Γ' veqsubst vr.
-  - intros ? h; inversion h; intros; split; intros; constructor.
-  - intros ???????? ih ? h; inversion h as [|?????? VΓad' VA' ]; subst.
+  - intros * h. inversion h; subst.
+    apply Specif.eq_sigT_uncurried_iff in H11; cbn in H11; destruct H11 as [eL e'].
+    assert (eq_refl = eL) as eeL by apply uip; destruct eeL; cbn in *.
+    apply Specif.eq_sigT_uncurried_iff in e'; cbn in e'; destruct e' as [eL' e].
+    assert (eq_refl = eL') as eeL' by apply uip; destruct eeL' ; cbn in *.
+    destruct e.
+    intros; split; intros; constructor.
+  - intros [Γ L] [Γ' L'] ?????? ih ? h; inversion h as [|?????? VΓad' VA' ]; subst.
+    apply Specif.eq_sigT_uncurried_iff in H18; cbn in H18; destruct H18 as [eΓA e'].
+    assert (eq_refl = eΓA) as eeΓA by apply uip; destruct eeΓA; cbn in *.
+    apply Specif.eq_sigT_uncurried_iff in e'; cbn in e'; destruct e' as [eΓA' e].
+    assert (eq_refl = eΓA') as eeΓA' by apply uip; destruct eeΓA' ; cbn in *.
+    destruct e.
     specialize (ih _ VΓad').
     intros; split; intros []; unshelve econstructor.
     1,2: now eapply ih.
@@ -39,7 +51,7 @@ Succeed Constraint v4 < u4.
 End VRIrrelevant.
 
 
-Lemma irrelevanceSubst {Γ Γ'} (VΓ VΓ' : [||-v Γ ≅ Γ']) {σ σ' Δ} (wfΔ wfΔ' : [|- Δ]) :
+Lemma irrelevanceSubst {Γ Γ'} (VΓ VΓ' : [||-v Γ ≅ Γ']) {Δ} (wfΔ wfΔ' : [|- Δ]) {ρF : Fweakening Δ Γ} {ρF' : Fweakening Δ Γ'} {σ σ'}:
   [Δ ||-v σ ≅ σ' : Γ | VΓ | wfΔ ] -> [Δ ||-v σ ≅ σ' : Γ | VΓ' | wfΔ'].
 Proof.
   eapply VRirrelevant; eapply VAd.adequate.
@@ -50,15 +62,15 @@ Lemma symSubst@{u1 u2 u3 u4} {Γ Γ'}
                      (VΓ  : VAdequate@{u3 u4} VR@{u1 u2 u3 u4} Γ Γ')
                      (VΓ'  : VAdequate@{u3 u4} VR@{u1 u2 u3 u4} Γ' Γ) :
   (* (VΓ VΓ' : [||-v Γ]) : *)
-  forall {σ σ' Δ} (wfΔ wfΔ' : [|- Δ]),
+  forall {Δ} (wfΔ wfΔ' : [|- Δ]) {ρF : Fweakening Δ Γ} {ρF' : Fweakening Δ Γ'} {σ σ'},
   [Δ ||-v σ ≅ σ' : Γ | VΓ | wfΔ ] -> [Δ ||-v σ' ≅ σ : _ | VΓ' | wfΔ'].
 Proof.
   revert VΓ'; induction Γ, Γ', VΓ using validity_rect; intros VΓ'.
   - rewrite (invValidityEmpty VΓ'). constructor.
   - pose proof (x := invValiditySnoc VΓ').
     destruct x as [lA'[ VΓ'' [VA' ->]]].
-    intros ????? [tleq hdeq].
-    pose (tleq' := IHVΓ VΓ'' _ _ _ wfΔ wfΔ' tleq).
+    intros ??????? [tleq hdeq].
+    pose (tleq' := IHVΓ VΓ'' _ wfΔ wfΔ' _ _ _ _ tleq).
     exists tleq'; now eapply symLR, irrLR.
 Qed.
 
@@ -66,7 +78,7 @@ Lemma symValidTy {Γ Γ' l A B} {VΓ : [||-v Γ ≅ Γ']} (VΓ' : [||-v Γ' ≅ 
   [Γ ||-v<l> A ≅ B | VΓ] -> [Γ' ||-v<l> B ≅ A | VΓ'].
 Proof.
   intros; constructor; intros; symmetry.
-  now unshelve (eapply validTyExt; tea; now eapply symSubst).
+  now unshelve (eapply (validTyExt (Γ:=Γ) (Γ':=Γ')); tea; now eapply symSubst).
 Qed.
 
 Lemma symValid {Γ Γ'} : [||-v Γ ≅ Γ'] -> [||-v Γ' ≅ Γ].
@@ -79,20 +91,20 @@ Qed.
 
 Lemma convSubst {Γ Γ' Γ''}
   (VΓ : [||-v Γ ≅ Γ']) (VΓ' : [||-v Γ ≅ Γ'']) :
-  forall {Δ} (wfΔ : [|- Δ]) {σ σ'},
+  forall {Δ} (wfΔ : [|- Δ]) {ρF : Fweakening Δ Γ} {ρF' : Fweakening Δ Γ'} {ρF'' : Fweakening Δ Γ''} {σ σ'},
   [Δ ||-v σ ≅ σ' : _ | VΓ | wfΔ ] ->
   [Δ ||-v σ ≅ σ' : _ | VΓ' | wfΔ ].
 Proof.
   revert Γ' VΓ; indValid VΓ'.
   - constructor.
-  - intros * ih ? VΓ0 *; pose proof (invValidity VΓ0) as (?&?&?&?&?&e&h); subst; cbn in h; subst.
-    intros [tl hd]; pose proof (tl' := ih _ _ _ _ _ _ tl).
+  - intros * ih [Γ'' L''] VΓ0 *; pose proof (invValidity VΓ0) as (?&?&?&?&?&e&eF&h); cbn in e,eF; subst; cbn in h; subst.
+    intros [tl hd]; pose proof (tl' := ih _ _ _ _ _ _ _ _ _ tl).
     exists tl'; now eapply irrLREqCum.
 Qed.
 
 Lemma convSubst' {Γ Γ' Γ''}
   (VΓ : [||-v Γ' ≅ Γ]) (VΓ' : [||-v Γ'' ≅ Γ]) :
-  forall {Δ} (wfΔ : [|- Δ]) {σ σ'},
+  forall {Δ} (wfΔ : [|- Δ]) {ρF : Fweakening Δ Γ} {ρF' : Fweakening Δ Γ'} {ρF'' : Fweakening Δ Γ''} {σ σ'},
   [Δ ||-v σ ≅ σ' : _ | VΓ' | wfΔ ] ->
   [Δ ||-v σ ≅ σ' : _ | VΓ | wfΔ ].
 Proof.
@@ -103,7 +115,8 @@ Qed.
 Lemma convValidTy {Γ Γ' Γ''}
   (VΓ : [||-v Γ ≅ Γ']) (VΓ' : [||-v Γ ≅ Γ'']) {l A B} :
   [_ ||-v<l> A ≅ B | VΓ] -> [_ ||-v<l> A ≅ B | VΓ'].
-Proof. intros VA; constructor; intros; eapply validTyExt; tea; now eapply convSubst. Qed.
+Proof. intros VA; constructor. intros. eapply (validTyExt (Γ:=Γ) (Γ':=Γ')); tea; now eapply convSubst.
+ Qed.
 
 Lemma convValidTy' {Γ Γ' Γ''}
   (VΓ : [||-v Γ ≅ Γ']) (VΓ' : [||-v Γ'' ≅ Γ']) {l A B} :
